@prefix : <http://www.semanticweb.org/byjus/ontologies/2024/6/KebiProject/> .
@prefix owl: <http://www.w3.org/2002/07/owl#> .
@prefix rdf: <http://www.w3.org/1999/02/22-rdf-syntax-ns#> .
@prefix xml: <http://www.w3.org/XML/1998/namespace> .
@prefix xsd: <http://www.w3.org/2001/XMLSchema#> .
@prefix rdfs: <http://www.w3.org/2000/01/rdf-schema#> .
@base <http://www.semanticweb.org/byjus/ontologies/2024/6/KebiProject/> .

<http://www.semanticweb.org/byjus/ontologies/2024/6/KebiProjectv2> rdf:type owl:Ontology .

#################################################################
#    Object Properties
#################################################################

###  http://www.semanticweb.org/byjus/ontologies/2024/6/KebiProject/menuHasMenuSection
:menuHasMenuSection rdf:type owl:ObjectProperty ;
                    rdfs:domain :Menu ;
                    rdfs:range :MenuSection ;
                    rdfs:comment "Links a menu to its various sections, such as appetizers, main courses, and desserts."@en .


###  http://www.semanticweb.org/byjus/ontologies/2024/6/KebiProject/menuItemHasFoodIngredient
:menuItemHasFoodIngredient rdf:type owl:ObjectProperty ;
                           rdfs:domain :MenuItem ;
                           rdfs:range :FoodIngredient ;
                           rdfs:comment "Specifies the food ingredients that make up a menu item."@en .


###  http://www.semanticweb.org/byjus/ontologies/2024/6/KebiProject/menuSectionHasMenuItem
:menuSectionHasMenuItem rdf:type owl:ObjectProperty ;
                        rdfs:domain :MenuSection ;
                        rdfs:range :MenuItem ;
                        rdfs:comment "Links a menu section to the menu items it includes."@en .


###  http://www.semanticweb.org/byjus/ontologies/2024/6/KebiProject/personHasPreferences
:personHasPreferences rdf:type owl:ObjectProperty ;
                      rdfs:domain :Person ;
                      rdfs:range :Preferences .


###  http://www.semanticweb.org/byjus/ontologies/2024/6/KebiProject/personIsClientOfRestaurant
:personIsClientOfRestaurant rdf:type owl:ObjectProperty ;
                            rdfs:domain :Person ;
                            rdfs:range :Restaurant ;
                            rdfs:comment "Associates a person with the restaurant they are a client of."@en .


###  http://www.semanticweb.org/byjus/ontologies/2024/6/KebiProject/preferenceHasAllergens
:preferenceHasAllergens rdf:type owl:ObjectProperty ;
                        rdfs:domain :Preferences ;
                        rdfs:range :Allergens .


###  http://www.semanticweb.org/byjus/ontologies/2024/6/KebiProject/preferenceHasCaloricLevel
:preferenceHasCaloricLevel rdf:type owl:ObjectProperty ;
                           rdfs:subPropertyOf owl:topObjectProperty ;
                           rdfs:domain :Preferences ;
                           rdfs:range :CaloricLevel .


###  http://www.semanticweb.org/byjus/ontologies/2024/6/KebiProject/preferenceHasDietaryPreference
:preferenceHasDietaryPreference rdf:type owl:ObjectProperty ;
                                rdfs:domain :Preferences ;
                                rdfs:range :DietaryPreference .


###  http://www.semanticweb.org/byjus/ontologies/2024/6/KebiProject/restaurantHasMenu
:restaurantHasMenu rdf:type owl:ObjectProperty ;
                   rdfs:domain :Restaurant ;
                   rdfs:range :Menu ;
                   rdfs:comment "Links a restaurant to the menus it offers."@en .


#################################################################
#    Data properties
#################################################################

###  http://www.semanticweb.org/byjus/ontologies/2024/6/KebiProject/foodIngredientHasAllergens
:foodIngredientHasAllergens rdf:type owl:DatatypeProperty ;
                            rdfs:domain :FoodIngredient ;
                            rdfs:range xsd:string ;
                            rdfs:comment "Lists the allergens present in a food ingredient, which may be important for dietary restrictions and health considerations."@en .


###  http://www.semanticweb.org/byjus/ontologies/2024/6/KebiProject/foodIngredientHasCalories
:foodIngredientHasCalories rdf:type owl:DatatypeProperty ;
                           rdfs:domain :FoodIngredient ;
                           rdfs:range xsd:nonNegativeInteger ;
                           rdfs:comment "Indicates the number of kilocalories contained in a specific quantity of the food ingredient. This data is used to calculate the total caloric content of a menu item."@en .


###  http://www.semanticweb.org/byjus/ontologies/2024/6/KebiProject/foodIngredientHasDietaryCategory
:foodIngredientHasDietaryCategory rdf:type owl:DatatypeProperty ;
                                  rdfs:subPropertyOf owl:topDataProperty ;
                                  rdfs:domain :FoodIngredient ;
                                  rdfs:range xsd:string .


###  http://www.semanticweb.org/byjus/ontologies/2024/6/KebiProject/foodIngredientHasName
:foodIngredientHasName rdf:type owl:DatatypeProperty ;
                       rdfs:domain :FoodIngredient ;
                       rdfs:range xsd:string ;
                       rdfs:comment "The name of the food ingredient. This property is used to identify and describe the ingredient in the context of a recipe or menu item."@en .


###  http://www.semanticweb.org/byjus/ontologies/2024/6/KebiProject/menuHasDescription
:menuHasDescription rdf:type owl:DatatypeProperty ;
                    rdfs:domain :Menu ;
                    rdfs:range xsd:string ;
                    rdfs:comment "A general description of the menu, providing an overview of the types of dishes offered and any special features."@en .


###  http://www.semanticweb.org/byjus/ontologies/2024/6/KebiProject/menuHasTitle
:menuHasTitle rdf:type owl:DatatypeProperty ;
              rdfs:domain :Menu ;
              rdfs:range xsd:string ;
              rdfs:comment "The title of the menu, used to distinguish it from other menus offered by the restaurant (e.g., 'Lunch Menu', 'Dinner Menu')."@en .


###  http://www.semanticweb.org/byjus/ontologies/2024/6/KebiProject/menuItemHasName
:menuItemHasName rdf:type owl:DatatypeProperty ;
                 rdfs:domain :MenuItem ;
                 rdfs:range xsd:string ;
                 rdfs:comment "The name of the menu item as it appears on the menu, used for identification and ordering purposes"@en .


###  http://www.semanticweb.org/byjus/ontologies/2024/6/KebiProject/menuSectionHasTitle
:menuSectionHasTitle rdf:type owl:DatatypeProperty ;
                     rdfs:domain :MenuSection ;
                     rdfs:range xsd:string .


###  http://www.semanticweb.org/byjus/ontologies/2024/6/KebiProject/personHasName
:personHasName rdf:type owl:DatatypeProperty ;
               rdfs:domain :Person ;
               rdfs:range xsd:string ;
               rdfs:comment "The full name of the person. This property is used for identifying and referencing individuals."@en .


###  http://www.semanticweb.org/byjus/ontologies/2024/6/KebiProject/restaurantHasName
:restaurantHasName rdf:type owl:DatatypeProperty ;
                   rdfs:domain :Restaurant ;
                   rdfs:range xsd:string ;
                   rdfs:comment "The official name of the restaurant, used for identification and branding purposes."@en .


###  http://www.semanticweb.org/byjus/ontologies/2024/6/KebiProjectv2#allergenHasName
:allergenHasName rdf:type owl:DatatypeProperty ;
                 rdfs:domain :Allergens ;
                 rdfs:range xsd:string .


###  http://www.semanticweb.org/byjus/ontologies/2024/6/KebiProjectv2#caloricLevelHasName
:caloricLevelHasName rdf:type owl:DatatypeProperty ;
                     rdfs:domain :CaloricLevel ;
                     rdfs:range xsd:string .


###  http://www.semanticweb.org/byjus/ontologies/2024/6/KebiProjectv2#dietaryPreferenceHasName
:dietaryPreferenceHasName rdf:type owl:DatatypeProperty ;
                          rdfs:domain :DietaryPreference ;
                          rdfs:range xsd:string .


#################################################################
#    Classes
#################################################################

###  http://www.semanticweb.org/byjus/ontologies/2024/6/KebiProject/Allergens
:Allergens rdf:type owl:Class ;
           rdfs:subClassOf :Preferences .


###  http://www.semanticweb.org/byjus/ontologies/2024/6/KebiProject/CaloricLevel
:CaloricLevel rdf:type owl:Class ;
              rdfs:subClassOf :Preferences ;
              rdfs:comment "Represents a range of caloric values for classifying food items based on their caloric content."@en .


###  http://www.semanticweb.org/byjus/ontologies/2024/6/KebiProject/DietaryPreference
:DietaryPreference rdf:type owl:Class ;
                   rdfs:subClassOf :Preferences ;
                   rdfs:comment "Describes an individual's dietary habits, restrictions, and preferences, including preferred caloric intake and allergens to avoid."@en .


###  http://www.semanticweb.org/byjus/ontologies/2024/6/KebiProject/FoodIngredient
:FoodIngredient rdf:type owl:Class ;
                rdfs:comment "Basic components or ingredients used in preparing menu items, with specific attributes such as calories and allergens." .


###  http://www.semanticweb.org/byjus/ontologies/2024/6/KebiProject/Menu
:Menu rdf:type owl:Class ;
      rdfs:comment "A collection of menu sections offered by a restaurant, detailing the available dishes and beverages."@en .


###  http://www.semanticweb.org/byjus/ontologies/2024/6/KebiProject/MenuItem
:MenuItem rdf:type owl:Class ;
          rdfs:comment "A specific dish or beverage offered in a menu, potentially composed of multiple food ingredients."@en .


###  http://www.semanticweb.org/byjus/ontologies/2024/6/KebiProject/MenuSection
:MenuSection rdf:type owl:Class ;
             rdfs:comment "A subsection of a menu, grouping similar items together, such as appetizers, main courses, or desserts."@en .


###  http://www.semanticweb.org/byjus/ontologies/2024/6/KebiProject/Person
:Person rdf:type owl:Class ;
        rdfs:comment "An individual, typically a client or customer, with specific dietary preferences and other personal attributes."@en .


###  http://www.semanticweb.org/byjus/ontologies/2024/6/KebiProject/Preferences
:Preferences rdf:type owl:Class .


###  http://www.semanticweb.org/byjus/ontologies/2024/6/KebiProject/Restaurant
:Restaurant rdf:type owl:Class ;
            rdfs:comment "An establishment that prepares and serves food and beverages to customers, offering various menus and dishes."@en .


#################################################################
#    Individuals
#################################################################

###  http://www.semanticweb.org/byjus/ontologies/2024/6/KebiProject/Appetizers
:Appetizers rdf:type owl:NamedIndividual ,
                     :MenuSection ;
            :menuSectionHasMenuItem :Tagliere_di_salumi_nostrani_servito_con_Gnocco_Fritto ;
            :menuSectionHasTitle "Appetizers"@en .


###  http://www.semanticweb.org/byjus/ontologies/2024/6/KebiProject/Coppa
:Coppa rdf:type owl:NamedIndividual ,
                :FoodIngredient ;
       :foodIngredientHasAllergens "" ;
       :foodIngredientHasCalories "300"^^xsd:nonNegativeInteger ;
       :foodIngredientHasDietaryCategory "Omnivore" ;
       :foodIngredientHasName "Coppa" .


###  http://www.semanticweb.org/byjus/ontologies/2024/6/KebiProject/Egg
:Egg rdf:type owl:NamedIndividual ,
              :Allergens ;
     :allergenHasName "Egg" .


###  http://www.semanticweb.org/byjus/ontologies/2024/6/KebiProject/Gluten
:Gluten rdf:type owl:NamedIndividual ,
                 :Allergens ;
        :allergenHasName "Gluten" .


###  http://www.semanticweb.org/byjus/ontologies/2024/6/KebiProject/Gnocco_Fritto
:Gnocco_Fritto rdf:type owl:NamedIndividual ,
                        :FoodIngredient ;
               :foodIngredientHasAllergens "Gluten" ;
               :foodIngredientHasCalories "300"^^xsd:nonNegativeInteger ;
               :foodIngredientHasDietaryCategory "Vegan" ;
               :foodIngredientHasName "Gnocco Fritto" .


###  http://www.semanticweb.org/byjus/ontologies/2024/6/KebiProject/High
:High rdf:type owl:NamedIndividual ,
               :CaloricLevel ;
      :caloricLevelHasName "High" .


###  http://www.semanticweb.org/byjus/ontologies/2024/6/KebiProject/Lactose
:Lactose rdf:type owl:NamedIndividual ,
                  :Allergens ;
         :allergenHasName "Lactose" .


###  http://www.semanticweb.org/byjus/ontologies/2024/6/KebiProject/Low
:Low rdf:type owl:NamedIndividual ,
              :CaloricLevel ;
     :caloricLevelHasName "Low" .


###  http://www.semanticweb.org/byjus/ontologies/2024/6/KebiProject/Martina
:Martina rdf:type owl:NamedIndividual ,
                  :Person ;
         :personHasPreferences :Martinas_Preferences ;
         :personIsClientOfRestaurant :Nero_Balsamico ;
         :personHasName "Martina" .


###  http://www.semanticweb.org/byjus/ontologies/2024/6/KebiProject/Martinas_Preferences
:Martinas_Preferences rdf:type owl:NamedIndividual ,
                               :Preferences ;
                      :preferenceHasAllergens :Lactose ;
                      :preferenceHasCaloricLevel :Medium ;
                      :preferenceHasDietaryPreference :Omnivore .


###  http://www.semanticweb.org/byjus/ontologies/2024/6/KebiProject/Medium
:Medium rdf:type owl:NamedIndividual ,
                 :CaloricLevel ;
        :caloricLevelHasName "Medium" .


###  http://www.semanticweb.org/byjus/ontologies/2024/6/KebiProject/Menu_SummerSpecial
:Menu_SummerSpecial rdf:type owl:NamedIndividual ,
                             :Menu ;
                    :menuHasMenuSection :Appetizers ;
                    :menuHasDescription "A summer special menu version" ;
                    :menuHasTitle "Menu Summer Special" .


###  http://www.semanticweb.org/byjus/ontologies/2024/6/KebiProject/Mortadella
:Mortadella rdf:type owl:NamedIndividual ,
                     :FoodIngredient ;
            :foodIngredientHasAllergens "Lactose" ;
            :foodIngredientHasCalories "350"^^xsd:nonNegativeInteger ;
            :foodIngredientHasDietaryCategory "Omnivore" ;
            :foodIngredientHasName "Mortadella" .


###  http://www.semanticweb.org/byjus/ontologies/2024/6/KebiProject/Nero_Balsamico
:Nero_Balsamico rdf:type owl:NamedIndividual ,
                         :Restaurant ;
                :restaurantHasMenu :Menu_SummerSpecial ;
                :restaurantHasName "Nero Balsamico" .


###  http://www.semanticweb.org/byjus/ontologies/2024/6/KebiProject/Nuts
:Nuts rdf:type owl:NamedIndividual ,
               :Allergens ;
      :allergenHasName "Nuts" .


###  http://www.semanticweb.org/byjus/ontologies/2024/6/KebiProject/Omnivore
:Omnivore rdf:type owl:NamedIndividual ,
                   :DietaryPreference ;
          :dietaryPreferenceHasName "Omnivore" .


###  http://www.semanticweb.org/byjus/ontologies/2024/6/KebiProject/Prosciutto_Crudo
:Prosciutto_Crudo rdf:type owl:NamedIndividual ,
                           :FoodIngredient ;
                  :foodIngredientHasAllergens "" ;
                  :foodIngredientHasCalories "250"^^xsd:nonNegativeInteger ;
                  :foodIngredientHasDietaryCategory "Omnivore" ;
                  :foodIngredientHasName "Prosciutto Crudo" .


###  http://www.semanticweb.org/byjus/ontologies/2024/6/KebiProject/Salame
:Salame rdf:type owl:NamedIndividual ,
                 :FoodIngredient ;
        :foodIngredientHasAllergens "" ;
        :foodIngredientHasCalories "400"^^xsd:nonNegativeInteger ;
        :foodIngredientHasDietaryCategory "Omnivore" ;
        :foodIngredientHasName "Salame" .


###  http://www.semanticweb.org/byjus/ontologies/2024/6/KebiProject/Tagliere_di_salumi_nostrani_servito_con_Gnocco_Fritto
:Tagliere_di_salumi_nostrani_servito_con_Gnocco_Fritto rdf:type owl:NamedIndividual ,
                                                                :MenuItem ;
                                                       :menuItemHasFoodIngredient :Coppa ,
                                                                                  :Gnocco_Fritto ,
                                                                                  :Mortadella ,
                                                                                  :Prosciutto_Crudo ,
                                                                                  :Salame ;
                                                       :menuItemHasName "Tagliere di salumi nostrani servito con Gnocco Fritto" .


###  http://www.semanticweb.org/byjus/ontologies/2024/6/KebiProject/Vegan
:Vegan rdf:type owl:NamedIndividual ,
                :DietaryPreference ;
       :dietaryPreferenceHasName "Vegan" .


###  http://www.semanticweb.org/byjus/ontologies/2024/6/KebiProject/Vegetarian
:Vegetarian rdf:type owl:NamedIndividual ,
                     :DietaryPreference ;
            :dietaryPreferenceHasName "Vegetarian" .


###  http://www.semanticweb.org/byjus/ontologies/2024/6/KebiProjectv2#Desserts
:Desserts rdf:type owl:NamedIndividual ,
                   :MenuSection ;
          :menuSectionHasTitle "Desserts" .


###  http://www.semanticweb.org/byjus/ontologies/2024/6/KebiProjectv2#First_Dish
:First_Dish rdf:type owl:NamedIndividual ,
                     :MenuSection ;
            :menuSectionHasTitle "First Dish" .


###  http://www.semanticweb.org/byjus/ontologies/2024/6/KebiProjectv2#Second_Dish
:Second_Dish rdf:type owl:NamedIndividual ,
                      :MenuSection ;
             :menuSectionHasTitle "Second Dish" .


###  http://www.semanticweb.org/byjus/ontologies/2024/6/KebiProjectv2#Side_Dish
:Side_Dish rdf:type owl:NamedIndividual ,
                    :MenuSection ;
           :menuSectionHasTitle "Side Dish" .


###  Generated by the OWL API (version 4.5.29.2024-05-13T12:11:03Z) https://github.com/owlcs/owlapi
